commit

AP/AP/FreshA1.lean
@@ -2,6 +2,269 @@ import AP.AP.DisjA
 
 namespace AP
 
+def State.HasDReenter (s : State) (fsp : FSP) : Prop :=
+  ∀ (a : AStrat), a.WF → s.aForallWinsDisj fsp a → ∃ (d : DStrat), d.WF ∧
+  ∃ n sd, DState sd ∧ sys.simulate (Strat.f ⟨a, d⟩) s n = (sd, 0) ∧ sd.aPos = s.aPos
+
+-----
+
+theorem AState.hasDReenter_of_not_aHwsDisj_insert_aPos {s fsp}
+[hs : AState s] (h₁ : ¬s.aHwsDisj (fsp.insert 1 s.aPos)) : s.HasDReenter fsp := by
+  intro a ha h₂
+  simp [State.aHwsDisj, State.aForallWinsDisj] at h₁
+  specialize h₁ a ha
+  choose d hd h₁ using h₁
+  use d, hd
+  simp [State.aWinsDisj] at h₁
+  choose n h₁ using h₁
+  specialize h₂ d hd
+  rw [State.aWinsDisj_iff] at h₂
+  choose h₂ h₃ using h₂
+  specialize h₂ n
+  generalize hr : sys.simulate (Strat.f ⟨a, d⟩) s n = r at h₂
+  rcases r with ⟨s₁, r⟩
+  dsimp at h₂; subst h₂
+  specialize h₁ s₁ hr
+  simp [FSP.hasLe, FSP.insert, FSP.insertSet] at h₁
+  choose k hk h₁ using h₁
+  specialize h₃ n
+  simp [hr, FSP.hasLe] at h₃
+  specialize h₃ k hk
+  split_ifs at h₁ with h₄
+  rotate_left; contradiction
+  subst h₄
+  simp [h₃] at h₁
+  have hs₁ : sys.WF s₁ := sys.wf_of_simulate_eq hr
+  replace hs₁ := s₁.aState_or_dState
+  rcases hs₁ with hs₁ | hs₁
+  rotate_left; use n, s₁
+  cases n
+  · simp at hk
+  nm n
+  have hr₁' := hr
+  rw [sys.simulate_add] at hr
+  simp at hr
+  rename' hr => hr₁
+  generalize hr : sys.simulate (Strat.f ⟨a, d⟩) s n = r at hr₁
+  rcases r with ⟨s', r⟩
+  dsimp at hr₁
+  obtain rfl : r = 0
+  · rw [Prod.snd_eq_of_eq_mk hr]
+    apply sys.simulate_snd_eq_zero_of_le_and_eq_zero # Prod.snd_eq_of_eq_mk hr₁' |>.symm
+    simp
+  simp at hr₁
+  have hs' : DState s'
+  · use sys.wf_of_simulate_eq hr
+    simp [State.aTurn_eq_of_tr' hr₁]
+  use n, s', hs', hr
+  rw [←DState.aPos_eq_of_tr hr₁, h₁]
+
+theorem AState.not_aHwsDisj_insert_aPos_of_hasDReenter {s fsp}
+[hs : AState s] (h : s.HasDReenter fsp) : ¬s.aHwsDisj (fsp.insert 1 s.aPos) := by
+  rintro ⟨a, ha, h₁⟩
+  specialize h a ha # State.aForallWinsDisj_of_aForallWinsDisj_insert h₁
+  choose d hd n sd hsd h₄ h₅ using h
+  specialize h₁ d hd n
+  choose sd' h₁ h₆ using h₁
+  simp [h₄] at h₁
+  subst h₁
+  simp [FSP.hasLe, FSP.insert, FSP.insertSet, h₅] at h₆
+  have h₇ : n ≠ 0
+  · rintro rfl
+    simp at h₄
+    subst h₄
+    cases hsd; nm H₁ H₂; simp at H₂
+  specialize h₆ 1 (by omega)
+  simp at h₆
+
+theorem AState.hasDReenter_iff_not_aHwsDisj_insert_aPos {s fsp}
+[hs : AState s] : s.HasDReenter fsp ↔ ¬s.aHwsDisj (fsp.insert 1 s.aPos) :=
+  ⟨not_aHwsDisj_insert_aPos_of_hasDReenter, hasDReenter_of_not_aHwsDisj_insert_aPos⟩
+
+theorem AState.hasDReenter_of_taken_subset {fsp s s'} [hs : AState s] [hs' : AState s']
+(h : s.HasDReenter fsp) (hpw : s'.pw = s.pw) (ht : s'.aTurn = s.aTurn)
+(hpa : s'.aPos = s.aPos) (h₁ : s.taken ⊆ s'.taken) : s'.HasDReenter fsp := by
+  rw [hasDReenter_iff_not_aHwsDisj_insert_aPos] at h ⊢
+  contrapose! h
+  symm at hpw ht hpa
+  have h₃ := @State.aHwsDisj_of_taken_subset (fsp.insert 1 s.aPos) s' s _ _
+    (by rwa [hpa]) hpw ht hpa h₁
+  exact State.aHwsDisj_of_aHwsDisj_insertSet h₃
+
+theorem AState.aHwsDisj_insert_one_aPos {s fsp} [hs : AState s]
+(h : s.aHwsDisj fsp) : s.aHwsDisj # fsp.insert 1 s.aPos := by
+  choose a ha h using h
+  by_contra h₀
+  rw [←AState.hasDReenter_iff_not_aHwsDisj_insert_aPos] at h₀
+  choose d hd n sd hsd h₂ h₃ using h₀ a ha h
+  generalize hM : (Set'.ofList # s.aPos.nbhd s.pw).erase s.aPos = M
+  generalize hN : (M \ sd.taken).size = N
+  induction N using Nat.strong_induction_on generalizing s d n sd
+  nm N ih
+  by_cases h₄ : N = 0
+  · clear ih
+    subst h₄ hM
+    simp at hN
+    rw [Set'.diff_eq_empty_iff_subset] at hN
+    specialize h d hd
+    rw [State.aWinsDisj_iff] at h
+    replace h := h.1
+    specialize h (n + 2)
+    rw [sys.simulate_add] at h
+    simp [h₂] at h
+    choose s₁ h₄ s₂ h₅ using h
+    have hs₁ := AState.of_tr h₄
+    simp at h₅
+    specialize hN s₂.aPos
+    simp at hN
+    rw [AState.tr_eq_some_iff] at h₅
+    rcases h₅ with ⟨⟨h₅, h₆, h₇⟩, rfl⟩
+    rw [DState.aPos_eq_of_tr h₄, h₃] at *
+    dsimp at hN
+    specialize hN h₅
+    rw [Point.dist_comm, pw_eq_of_tr h₄, State.pw_eq_of_simulate_eq h₂] at h₇
+    specialize hN h₇
+    apply h₆
+    apply Set'.mem_of_subset _ hN
+    exact taken_subset_of_tr h₄
+  obtain ⟨p, hp₁, hp₂, hp₃⟩ : ∃ p, p ∉ sd.taken ∧ p.dist sd.aPos ≤ sd.pw ∧ sd.aPos ≠ p
+  · replace h₄ : M \ sd.taken ≠ ∅
+    · rw [←hN] at h₄
+      simp at h₄
+      exact h₄
+    replace h₄ := Set'.exi_mem_of_ne_empty h₄
+    choose p h₄ using h₄
+    simp [←hM] at h₄
+    use p
+    obtain ⟨⟨hp₃, hp₂⟩, hp₁⟩ := h₄
+    rw [h₃]
+    refine ⟨hp₁, ?_, hp₃⟩
+    rwa [Point.dist_comm, State.pw_eq_of_simulate_eq h₂]
+  have h₅ : sys.validTr sd p
+  · rw [DState.validTr_iff]
+    use hp₃
+  choose sa h₅ using h₅
+  have hsa := AState.of_tr h₅
+  have h₆ : sd.aForallWinsDisj fsp a
+  · have h := State.aForallWinsDisj_of_simulate_eq h h₂
+    exact State.aForallWinsDisj_of_aForallWinsDisj_offset h
+  replace h₆ := DState.tr_of_aForallWinsDisj h₆ h₅
+  replace h₆ := State.aForallWinsDisj_of_aForallWinsDisj_next h₆
+  have h₇ : s.taken ⊆ sa.taken
+  · apply Set'.subset_trans _ # taken_subset_of_tr h₅
+    exact taken_subset_of_reachable # sys.reachable_of_simulate_eq h₂
+  have h₈ : sa.HasDReenter fsp
+  · apply AState.hasDReenter_of_taken_subset h₀
+    · rw [pw_eq_of_tr h₅, State.pw_eq_of_simulate_eq h₂]
+    · simp
+    · rwa [DState.aPos_eq_of_tr h₅]
+    · exact h₇
+  choose d₁ hd₁ n₁ sd₁ hsd₁ H₁ H₂ using h₈ a ha h₆
+  generalize hN₁ : (M \ sd₁.taken).size = N₁
+  have H₄ : sys.Reachable sd sd₁
+  · apply sys.reachable_of_tr h₅ |>.trans
+    exact sys.reachable_of_simulate_eq H₁
+  have H₃ := taken_subset_of_reachable H₄
+  have H₅ : N₁ < N
+  · rw [←hN, ←hN₁]
+    apply Set'.size_lt_of_ssubset
+    apply Set'.diff_ssubset_of_right H₃
+    use p
+    simp [←hM, hp₁, ←h₃, hp₃, ←State.pw_eq_of_simulate_eq h₂]
+    rw [Point.dist_comm]
+    use hp₂
+    apply State.mem_taken_of_reachable # sys.reachable_of_simulate_eq H₁
+    exact DState.mem_taken_of_tr h₅
+  apply @ih N₁ H₅ sa hsa h₆ h₈ d₁ hd₁ n₁ sd₁ hsd₁ H₁ H₂ _ hN₁
+  rw [DState.aPos_eq_of_tr h₅, h₃]
+  rw [pw_eq_of_tr h₅, State.pw_eq_of_simulate_eq h₂]
+  exact hM
+
+theorem DState.forall_tr_of_aHwsDisj {s fsp} [hs : DState s] (h : s.aHwsDisj fsp) :
+∀ p s', sys.tr s p = some s' → s'.aHwsDisj fsp.next :=
+  λ _ _ h₁ => tr_of_aHwsDisj h h₁
+
+theorem DState.forall_tr_exi_aForallWinsDisj_of_aHwsDisj {s fsp} [hs : DState s]
+(h : s.aHwsDisj fsp) : ∀ p, ∃ (a : AStrat), a.WF ∧
+∀ s', sys.tr s p = some s' → s'.aForallWinsDisj fsp.next a := by
+  intro p
+  have h₁ := DState.forall_tr_of_aHwsDisj h p
+  cases h₂ : sys.tr s p
+  · use default, inferInstance; simp
+  nm s₁
+  simp
+  specialize h₁ s₁ h₂
+  exact h₁
+
+theorem DState.aHwsDisj_iff_forall_tr_exi_aForallWinsDisj {s fsp} [hs : DState s] :
+s.aHwsDisj fsp ↔ ∀ p, ∃ (a : AStrat), a.WF ∧
+∀ s', sys.tr s p = some s' → s'.aForallWinsDisj fsp.next a := by
+  use forall_tr_exi_aForallWinsDisj_of_aHwsDisj
+  intro h
+  choose A hA h using h
+  use .mk # λ s₁ => A (s₁.getMoveAt s).iget |>.f s₁
+  use inferInstance
+  intro d hd
+  obtain ⟨s', h₁⟩ := d.validTr s
+  specialize h _ _ h₁
+  intro n
+  cases n
+  · simp
+    specialize h d hd 0
+    simp at h
+    rw [←DState.aPos_eq_of_tr h₁]
+    exact h.1
+  nm n
+  specialize h d hd n
+  have hs' := AState.of_tr h₁
+  choose s₁ h₂ h₃ using h
+  use s₁
+  split_ands
+  rotate_left
+  · contrapose! h₃
+    rwa [FSP.hasLe_next]
+  simp [h₁]
+  rw [←h₂]
+  apply simulate_congr _ # by simp
+  intro k hk sa hsa H₁ H₂ H₃
+  simp
+  have H₄ : sa.getMoveAt s = some (d.f s)
+  · apply getMoveAt_eq_some_of_tr_and_reachable h₁
+    exact sys.reachable_of_simulate_eq H₂
+  simp [H₄, Option.iget, AStrat.validTr H₃]
+
+theorem DState.aHwsDisj_iff_forall_tr {s fsp} [hs : DState s] :
+s.aHwsDisj fsp ↔ ∀ p s', sys.tr s p = some s' → s'.aHwsDisj fsp.next := by
+  rw [aHwsDisj_iff_forall_tr_exi_aForallWinsDisj]
+  unfold State.aHwsDisj
+  apply forall_congr'; intro p
+  cases h : sys.tr s p
+  · simp
+    use default
+    infer_instance
+  nm s₁
+  simp
+
+theorem DState.aHwsDisj_insert_two_aPos {s fsp} [hs : DState s]
+(h : s.aHwsDisj fsp) : s.aHwsDisj # fsp.insert 2 s.aPos := by
+  rw [DState.aHwsDisj_iff_forall_tr]
+  intro p s' h₁
+  have hs' := AState.of_tr h₁
+  replace h := tr_of_aHwsDisj h h₁
+  replace h := AState.aHwsDisj_insert_one_aPos h
+  rwa [FSP.next_insert_succ, ←DState.aPos_eq_of_tr h₁]
+
+theorem State.aHwsDisj_insert_two_aPos {s fsp} [hs : sys.WF s]
+(h : s.aHwsDisj fsp) : s.aHwsDisj # fsp.insert 2 s.aPos := by
+  replace hs := s.aState_or_dState
+  rcases hs with hs | hs
+  · apply State.aHwsDisj_insert_of_le
+    . exact hs.aHwsDisj_insert_one_aPos h
+    · simp
+  · exact DState.aHwsDisj_insert_two_aPos h
+
+-- #check 0 #exit
+
 theorem AState.aHwsDisj_nbhd_pw {s : State} {fsp : FSP} [hs : AState s]
 (h : s.aHwsDisj fsp) : s.aHwsDisj # fsp.insertSet 3 # s.aPos.nbhd s.pw |>.toSet := by
   --   obtain ⟨a, Ha, h⟩ := h
